another way to think of the Fs spec; this time with non-determinism

Fs.v
@@ -1,6 +1,7 @@
 Require Import List.
 Require Import CpdtTactics.
 Require Import Arith.
+Import ListNotations.
 
 (* Take a trivial history of file operations (e.g., [ (Read, 0) (Write, 1)
 (Crash, 0) (Sync, 0) (Read, 1)]), and say whether it is legal.  Perhaps a proof
@@ -17,6 +18,8 @@ Inductive event : Set :=
   | Sync: event
   | Crash: event.
 
+Definition history := list event.
+
 (* To define what crash and sync do, file has two values: its in-memory value
 and its on-disk value. Only 1 file with a single integer has content. *)
 
@@ -24,8 +27,6 @@ Record file : Type := mkfile {
   Vmem : nat;
   Vdisk: nat
 }.
-
-Definition history := list event.
 
 (* A event returns whether its return value was legal and what the file's state
 is after the processing the event. Write updates the in-memory state. Sync
@@ -62,3 +63,92 @@ Eval simpl in legal ((Write 1) :: Sync :: (Read 0) :: nil) (mkfile 0 0).
 Eval simpl in legal ((Write 1) :: (Read 1) :: Crash :: nil) (mkfile 0 0).
 Eval simpl in legal ((Write 1) :: (Read 1) :: Crash :: (Read 0) :: nil) (mkfile 0 0).
 Eval simpl in legal ((Write 1) :: (Read 1) :: Crash :: (Read 1) :: nil) (mkfile 0 0).
+
+(* An alternative definition of legal histories.  Note that this
+ * definition treats histories "backwards": writing and then reading
+ * a file is represented by: (Read 1) :: (Write 1) :: nil.
+ *)
+
+(* (last_wrote h n) means n was the last data written *)
+Inductive last_wrote: history -> nat -> Prop :=
+  | last_wrote_read:
+    forall (h:history) (n:nat) (rn:nat),
+    last_wrote h n -> last_wrote ((Read rn) :: h) n
+  | last_wrote_write:
+    forall (h:history) (n:nat),
+    last_wrote ((Write n) :: h) n
+  | last_wrote_sync:
+    forall (h:history) (n:nat),
+    last_wrote h n -> last_wrote (Sync :: h) n
+  | last_wrote_crash:
+    forall (h:history) (n:nat),
+    last_wrote h n -> last_wrote (Crash :: h) n.
+
+(* (wrote_since_sync h n) means n was either the last thing written before
+   the last sync, or was written after the last sync *)
+Inductive wrote_since_sync: history -> nat -> Prop :=
+  | wrote_since_sync_read:
+    forall (h:history) (n:nat) (rn:nat),
+    wrote_since_sync h n -> wrote_since_sync ((Read rn) :: h) n
+  | wrote_since_sync_write_1:
+    forall (h:history) (n:nat),
+    wrote_since_sync ((Write n) :: h) n
+  | wrote_since_sync_write_2:
+    forall (h:history) (n:nat) (wn:nat),
+    wrote_since_sync h n -> wrote_since_sync ((Write wn) :: h) n
+  | wrote_since_sync_sync:
+    forall (h:history) (n:nat),
+    last_wrote h n -> wrote_since_sync (Sync :: h) n
+  | wrote_since_sync_crash:
+    (* XXX
+       One sensible requirement that this fails to model is that,
+       once a system crashes, each file gets a well-defined value.
+       So this allows a file to keep flip-flopping between values,
+       across many crashes, until it's finally Sync'ed.
+     *)
+    forall (h:history) (n:nat),
+    wrote_since_sync h n -> wrote_since_sync (Crash :: h) n.
+
+(* (could_read h n) means n could be the return value of a read *)
+Inductive could_read: history -> nat -> Prop :=
+  | could_read_read:
+    forall (h:history) (n:nat) (rn:nat),
+    could_read h n -> could_read ((Read rn) :: h) n
+  | could_read_write:
+    forall (h:history) (n:nat),
+    could_read ((Write n) :: h) n
+  | could_read_sync:
+    forall (h:history) (n:nat),
+    could_read h n -> could_read (Sync :: h) n
+  | could_read_crash:
+    forall (h:history) (n:nat),
+    wrote_since_sync h n -> could_read (Crash :: h) n.
+
+Inductive legal2: history -> Prop :=
+  | legal2_read:
+    forall (h:history) (n:nat),
+    could_read h n ->
+    legal2 h -> legal2 ((Read n) :: h)
+  | legal2_write:
+    forall (h:history) (n:nat),
+    legal2 h -> legal2 ((Write n) :: h)
+  | legal2_sync:
+    forall (h:history),
+    legal2 h -> legal2 (Sync :: h)
+  | legal2_crash:
+    forall (h:history),
+    legal2 h -> legal2 (Crash :: h)
+  | legal2_nil:
+    legal2 nil.
+
+Theorem test_legal2_1:
+  legal2 [ Read 1 ; Crash ; Write 0 ; Sync ; Write 1 ].
+Proof.
+  repeat constructor.
+Qed.
+
+Theorem test_legal2_0:
+  legal2 [ Read 0 ; Crash ; Write 0 ; Sync ; Write 1 ].
+Proof.
+  repeat constructor.
+Qed.
